staged/HeapF_FO.v
@@ -1,0 +1,689 @@
+From SLF Require Export LibString LibCore.
+From SLF Require Export LibSepTLCbuffer.
+From SLF Require LibSepSimpl.
+
+From Staged Require Import LibFmap.
+
+Module Type HeapParams.
+  Parameter loc : Type.
+  Parameter val : Type.
+  Parameter null : loc.
+  Parameter pprop : Type. (* FO encoding of pure proposition *)
+  Parameter interp_pprop : pprop -> Prop. (* How to interpret a pure proposition *)
+End HeapParams.
+
+Module HeapSetup (P : HeapParams).
+
+Import P.
+
+Set Implicit Arguments.
+
+Definition heap : Type := fmap loc val.
+
+(* ################################################################# *)
+(** * Heap Predicates *)
+
+(** We next define heap predicates and establish their properties. All this
+    material is wrapped in a module, allowing us to instantiate the functor from
+    chapter [LibSepSimpl] that defines the tactic [xsimpl]. *)
+Module SepSimplArgs.
+
+(* ================================================================= *)
+(** ** Hprop and Entailment *)
+
+Declare Scope hprop_scope.
+Open Scope hprop_scope.
+
+(** The type of heap predicates is named [hprop]. *)
+
+Inductive hprop : Type :=
+| hempty : hprop
+| hpure : pprop -> hprop
+| hsingle : loc -> val -> hprop
+| hstar : hprop -> hprop -> hprop.
+
+(* Should give a definition here *)
+Parameter interp_hprop : heap -> hprop -> Prop.
+
+(** Entailment for heap predicates, written [H1 ==> H2]. This entailment
+    is linear. *)
+
+Definition himpl (hp1 hp2 : hprop) : Prop :=
+  forall h, interp_hprop h hp1 -> interp_hprop h hp2.
+
+Notation "H1 ==> H2" := (himpl H1 H2) (at level 55) : hprop_scope.
+
+(* ================================================================= *)
+(** ** Definition of Heap Predicates *)
+
+(** The core heap predicates are defined next, together with the
+    associated notation:
+
+    - [\[]] denotes the empty heap predicate
+    - [\[P]] denotes a pure fact
+    - [\Top] denotes the true heap predicate (affine)
+    - [p ~~> v] denotes a singleton heap
+    - [H1 \* H2] denotes the separating conjunction
+    - [Q1 \*+ H2] denotes the separating conjunction extending a postcondition
+    - [\exists x, H] denotes an existential quantifier
+    - [\forall x, H] denotes a universal quantifier
+    - [H1 \-* H2] denotes a magic wand between heap predicates
+    - [Q1 \--* Q2] denotes a magic wand between postconditions. *)
+
+Notation "\[]" := (hempty) (at level 0) : hprop_scope.
+
+Notation "\[ pp ]" := (hpure pp) (at level 0) : hprop_scope.
+
+Notation "l '~~>' v" := (hsingle l v) (at level 32) : hprop_scope.
+
+Notation "hp1 '\*' hp2" := (hstar hp1 hp2) (at level 41, right associativity) : hprop_scope.
+
+(* ================================================================= *)
+(** ** Basic Properties of Separation Logic Operators *)
+
+(* ----------------------------------------------------------------- *)
+(** *** Tactic for Automation *)
+
+(** We set up [auto] to process goals of the form [h1 = h2] by calling
+    [fmap_eq], which proves equality modulo associativity and commutativity. *)
+
+#[global] Hint Extern 1 (_ = _ :> heap) => fmap_eq.
+
+(** We also set up [auto] to process goals of the form [Fmap.disjoint h1 h2]
+    by calling the tactic [fmap_disjoint], which essentially normalizes all
+    disjointness goals and hypotheses, split all conjunctions, and invokes
+    proof search with a base of hints specified in [LibSepFmap.v]. *)
+
+Import Fmap.DisjointHints.
+
+Tactic Notation "fmap_disjoint_pre" :=
+  subst; rew_disjoint; jauto_set.
+
+#[global] Hint Extern 1 (Fmap.disjoint _ _) => fmap_disjoint_pre.
+
+(* ----------------------------------------------------------------- *)
+(** *** Properties of [himpl] and [qimpl] *)
+
+Lemma himpl_refl : forall H,
+  H ==> H.
+Proof using. introv M. auto. Qed.
+
+#[global] Hint Resolve himpl_refl.
+
+Lemma himpl_trans : forall H2 H1 H3,
+  (H1 ==> H2) ->
+  (H2 ==> H3) ->
+  (H1 ==> H3).
+Proof using. introv M1 M2. unfolds* himpl. Qed.
+
+Lemma himpl_trans_r : forall H2 H1 H3,
+   H2 ==> H3 ->
+   H1 ==> H2 ->
+   H1 ==> H3.
+Proof using. introv M1 M2. applys* himpl_trans M2 M1. Qed.
+
+(* ----------------------------------------------------------------- *)
+(** *** Properties of [hempty] *)
+
+Lemma hempty_intro :
+  interp_hprop Fmap.empty \[].
+Proof using. unfolds*. Qed.
+
+Lemma hempty_inv : forall h,
+  \[] h ->
+  h = Fmap.empty.
+Proof using. auto. Qed.
+
+(* ----------------------------------------------------------------- *)
+(** *** Properties of [hstar] *)
+
+Lemma hstar_intro : forall H1 H2 h1 h2,
+  H1 h1 ->
+  H2 h2 ->
+  Fmap.disjoint h1 h2 ->
+  (H1 \* H2) (Fmap.union h1 h2).
+Proof using. intros. exists~ h1 h2. Qed.
+
+Lemma hstar_inv : forall H1 H2 h,
+  (H1 \* H2) h ->
+  exists h1 h2, H1 h1 /\ H2 h2 /\ Fmap.disjoint h1 h2 /\ h = Fmap.union h1 h2.
+Proof using. introv M. applys M. Qed.
+
+Lemma hstar_comm : forall H1 H2,
+   H1 \* H2 = H2 \* H1.
+Proof using.
+  applys hprop_op_comm. unfold hprop, hstar. intros H1 H2.
+  intros h (h1&h2&M1&M2&D&U). rewrite~ Fmap.union_comm_of_disjoint in U.
+  exists* h2 h1.
+Qed.
+
+Lemma hstar_assoc : forall H1 H2 H3,
+  (H1 \* H2) \* H3 = H1 \* (H2 \* H3).
+Proof using.
+  intros H1 H2 H3. applys himpl_antisym; intros h.
+  { intros (h'&h3&(h1&h2&M3&M4&D'&U')&M2&D&U). subst h'.
+    exists h1 (h2 \+ h3). splits~. { applys* hstar_intro. } }
+  { intros (h1&h'&M1&(h2&h3&M3&M4&D'&U')&D&U). subst h'.
+    exists (h1 \+ h2) h3. splits~. { applys* hstar_intro. } }
+Qed.
+
+Lemma hstar_hempty_l : forall H,
+  \[] \* H = H.
+Proof using.
+  intros. applys himpl_antisym; intros h.
+  { intros (h1&h2&M1&M2&D&U). forwards E: hempty_inv M1. subst.
+    rewrite~ Fmap.union_empty_l. }
+  { intros M. exists (Fmap.empty:heap) h. splits~. { applys hempty_intro. } }
+Qed.
+
+Lemma hstar_hempty_r : forall H,
+  H \* \[] = H.
+Proof using.
+  applys neutral_r_of_comm_neutral_l. applys~ hstar_comm. applys~ hstar_hempty_l.
+Qed.
+
+Lemma hstar_hexists : forall A (J:A->hprop) H,
+  (hexists J) \* H = hexists (fun x => (J x) \* H).
+Proof using.
+  intros. applys himpl_antisym; intros h.
+  { intros (h1&h2&(x&M1)&M2&D&U). exists~ x h1 h2. }
+  { intros (x&(h1&h2&M1&M2&D&U)). exists h1 h2. splits~. { exists~ x. } }
+Qed.
+
+Lemma hstar_hforall : forall H A (J:A->hprop),
+  (hforall J) \* H ==> hforall (J \*+ H).
+Proof using.
+  intros. intros h M. destruct M as (h1&h2&M1&M2&D&U). intros x. exists~ h1 h2.
+Qed.
+
+Lemma himpl_frame_l : forall H2 H1 H1',
+  H1 ==> H1' ->
+  (H1 \* H2) ==> (H1' \* H2).
+Proof using. introv W (h1&h2&?). exists* h1 h2. Qed.
+
+Lemma himpl_frame_r : forall H1 H2 H2',
+  H2 ==> H2' ->
+  (H1 \* H2) ==> (H1 \* H2').
+Proof using.
+  introv M. do 2 rewrite (@hstar_comm H1). applys~ himpl_frame_l.
+Qed.
+
+Lemma himpl_frame_lr : forall H1 H1' H2 H2',
+  H1 ==> H1' ->
+  H2 ==> H2' ->
+  (H1 \* H2) ==> (H1' \* H2').
+Proof using.
+  introv M1 M2. applys himpl_trans. applys~ himpl_frame_l M1. applys~ himpl_frame_r.
+Qed.
+
+Lemma himpl_hstar_trans_l : forall H1 H2 H3 H4,
+  H1 ==> H2 ->
+  H2 \* H3 ==> H4 ->
+  H1 \* H3 ==> H4.
+Proof using.
+  introv M1 M2. applys himpl_trans M2. applys himpl_frame_l M1.
+Qed.
+
+Lemma himpl_hstar_trans_r : forall H1 H2 H3 H4,
+  H1 ==> H2 ->
+  H3 \* H2 ==> H4 ->
+  H3 \* H1 ==> H4.
+Proof using.
+  introv M1 M2. applys himpl_trans M2. applys himpl_frame_r M1.
+Qed.
+
+(* ----------------------------------------------------------------- *)
+(** ***  Properties of [hpure] *)
+
+Lemma hpure_intro : forall P,
+  P ->
+  \[P] Fmap.empty.
+Proof using. introv M. exists M. unfolds*. Qed.
+
+Lemma hpure_inv : forall P h,
+  \[P] h ->
+  P /\ h = Fmap.empty.
+Proof using. introv (p&M). split~. Qed.
+
+Lemma hstar_hpure_l : forall P H h,
+  (\[P] \* H) h = (P /\ H h).
+Proof using.
+  intros. apply prop_ext. unfold hpure.
+  rewrite hstar_hexists. rewrite* hstar_hempty_l.
+  iff (p&M) (p&M). { split~. } { exists~ p. }
+Qed.
+
+Lemma hstar_hpure_r : forall P H h,
+  (H \* \[P]) h = (H h /\ P).
+Proof using.
+  intros. rewrite hstar_comm. rewrite hstar_hpure_l. apply* prop_ext.
+Qed.
+
+Lemma himpl_hstar_hpure_r : forall P H H',
+  P ->
+  (H ==> H') ->
+  H ==> (\[P] \* H').
+Proof using. introv HP W. intros h K. rewrite* hstar_hpure_l. Qed.
+
+Lemma hpure_inv_hempty : forall P h,
+  \[P] h ->
+  P /\ \[] h.
+Proof using.
+  introv M. rewrite <- hstar_hpure_l. rewrite~ hstar_hempty_r.
+Qed.
+
+Lemma hpure_intro_hempty : forall P h,
+  \[] h ->
+  P ->
+  \[P] h.
+Proof using.
+  introv M N. rewrite <- (hstar_hempty_l \[P]). rewrite~ hstar_hpure_r.
+Qed.
+
+Lemma himpl_hempty_hpure : forall P,
+  P ->
+  \[] ==> \[P].
+Proof using. introv HP. intros h Hh. applys* hpure_intro_hempty. Qed.
+
+Lemma himpl_hstar_hpure_l : forall P H H',
+  (P -> H ==> H') ->
+  (\[P] \* H) ==> H'.
+Proof using.
+  introv W Hh. rewrite hstar_hpure_l in Hh. applys* W.
+Qed.
+
+Lemma hempty_eq_hpure_true :
+  \[] = \[True].
+Proof using.
+  applys himpl_antisym; intros h M.
+  { applys* hpure_intro_hempty. }
+  { forwards*: hpure_inv_hempty M. }
+Qed.
+
+Lemma hfalse_hstar_any : forall H,
+  \[False] \* H = \[False].
+Proof using.
+  intros. applys himpl_antisym; intros h; rewrite hstar_hpure_l; intros M.
+  { false*. } { lets: hpure_inv_hempty M. false*. }
+Qed.
+
+(* ----------------------------------------------------------------- *)
+(** *** Properties of [hexists] *)
+
+Lemma hexists_intro : forall A (x:A) (J:A->hprop) h,
+  J x h ->
+  (hexists J) h.
+Proof using. intros. exists~ x. Qed.
+
+Lemma hexists_inv : forall A (J:A->hprop) h,
+  (hexists J) h ->
+  exists x, J x h.
+Proof using. intros. destruct H as [x H]. exists~ x. Qed.
+
+Lemma himpl_hexists_l : forall A H (J:A->hprop),
+  (forall x, J x ==> H) ->
+  (hexists J) ==> H.
+Proof using. introv W. intros h (x&Hh). applys* W. Qed.
+
+Lemma himpl_hexists_r : forall A (x:A) H J,
+  (H ==> J x) ->
+  H ==> (hexists J).
+Proof using. introv W. intros h. exists x. apply~ W. Qed.
+
+Lemma himpl_hexists : forall A (J1 J2:A->hprop),
+  J1 ===> J2 ->
+  hexists J1 ==> hexists J2.
+Proof using.
+  introv W. applys himpl_hexists_l. intros x. applys himpl_hexists_r W.
+Qed.
+
+(* ----------------------------------------------------------------- *)
+(** *** Properties of [hforall] *)
+
+Lemma hforall_intro : forall A (J:A->hprop) h,
+  (forall x, J x h) ->
+  (hforall J) h.
+Proof using. introv M. applys* M. Qed.
+
+Lemma hforall_inv : forall A (J:A->hprop) h,
+  (hforall J) h ->
+  forall x, J x h.
+Proof using. introv M. applys* M. Qed.
+
+Lemma himpl_hforall_r : forall A (J:A->hprop) H,
+  (forall x, H ==> J x) ->
+  H ==> (hforall J).
+Proof using. introv M. intros h Hh x. apply~ M. Qed.
+
+Lemma himpl_hforall_l : forall A x (J:A->hprop) H,
+  (J x ==> H) ->
+  (hforall J) ==> H.
+Proof using. introv M. intros h Hh. apply~ M. Qed.
+
+Lemma hforall_specialize : forall A (x:A) (J:A->hprop),
+  (hforall J) ==> (J x).
+Proof using. intros. applys* himpl_hforall_l x. Qed.
+
+Lemma himpl_hforall : forall A (J1 J2:A->hprop),
+  J1 ===> J2 ->
+  hforall J1 ==> hforall J2.
+Proof using.
+  introv W. applys himpl_hforall_r. intros x. applys himpl_hforall_l W.
+Qed.
+
+(* ----------------------------------------------------------------- *)
+(** *** Properties of [hwand] *)
+
+Lemma hwand_equiv : forall H0 H1 H2,
+  (H0 ==> H1 \-* H2) <-> (H1 \* H0 ==> H2).
+Proof using.
+  unfold hwand. iff M.
+  { rewrite hstar_comm. applys himpl_hstar_trans_l (rm M).
+    rewrite hstar_hexists. applys himpl_hexists_l. intros H.
+    rewrite (hstar_comm H). rewrite hstar_assoc.
+    rewrite (hstar_comm H H1). applys~ himpl_hstar_hpure_l. }
+  { applys himpl_hexists_r H0.
+    rewrite <- (hstar_hempty_r H0) at 1.
+    applys himpl_frame_r. applys himpl_hempty_hpure M. }
+Qed.
+
+Lemma himpl_hwand_r : forall H1 H2 H3,
+  H2 \* H1 ==> H3 ->
+  H1 ==> (H2 \-* H3).
+Proof using. introv M. rewrite~ hwand_equiv. Qed.
+
+Lemma himpl_hwand_r_inv : forall H1 H2 H3,
+  H1 ==> (H2 \-* H3) ->
+  H2 \* H1 ==> H3.
+Proof using. introv M. rewrite~ <- hwand_equiv. Qed.
+
+Lemma hwand_cancel : forall H1 H2,
+  H1 \* (H1 \-* H2) ==> H2.
+Proof using. intros. applys himpl_hwand_r_inv. applys himpl_refl. Qed.
+
+Arguments hwand_cancel : clear implicits.
+
+Lemma himpl_hempty_hwand_same : forall H,
+  \[] ==> (H \-* H).
+Proof using. intros. apply himpl_hwand_r. rewrite~ hstar_hempty_r. Qed.
+
+Lemma hwand_hempty_l : forall H,
+  (\[] \-* H) = H.
+Proof using.
+  intros. applys himpl_antisym.
+  { rewrite <- hstar_hempty_l at 1. applys hwand_cancel. }
+  { rewrite hwand_equiv. rewrite~ hstar_hempty_l. }
+Qed.
+
+Lemma hwand_hpure_l : forall P H,
+  P ->
+  (\[P] \-* H) = H.
+Proof using.
+  introv HP. applys himpl_antisym.
+  { lets K: hwand_cancel \[P] H. applys himpl_trans K.
+    applys* himpl_hstar_hpure_r. }
+  { rewrite hwand_equiv. applys* himpl_hstar_hpure_l. }
+Qed.
+
+Lemma hwand_curry : forall H1 H2 H3,
+  (H1 \* H2) \-* H3 ==> H1 \-* (H2 \-* H3).
+Proof using.
+  intros. apply himpl_hwand_r. apply himpl_hwand_r.
+  rewrite <- hstar_assoc. rewrite (hstar_comm H1 H2).
+  applys hwand_cancel.
+Qed.
+
+Lemma hwand_uncurry : forall H1 H2 H3,
+  H1 \-* (H2 \-* H3) ==> (H1 \* H2) \-* H3.
+Proof using.
+  intros. rewrite hwand_equiv. rewrite (hstar_comm H1 H2).
+  rewrite hstar_assoc. applys himpl_hstar_trans_r.
+  { applys hwand_cancel. } { applys hwand_cancel. }
+Qed.
+
+Lemma hwand_curry_eq : forall H1 H2 H3,
+  (H1 \* H2) \-* H3 = H1 \-* (H2 \-* H3).
+Proof using.
+  intros. applys himpl_antisym.
+  { applys hwand_curry. }
+  { applys hwand_uncurry. }
+Qed.
+
+Lemma hwand_inv : forall h1 h2 H1 H2,
+  (H1 \-* H2) h2 ->
+  H1 h1 ->
+  Fmap.disjoint h1 h2 ->
+  H2 (h1 \u h2).
+Proof using.
+  introv M2 M1 D. unfolds hwand. lets (H0&M3): hexists_inv M2.
+  lets (h0&h3&P1&P3&D'&U): hstar_inv M3. lets (P4&E3): hpure_inv P3.
+  subst h2 h3. rewrite union_empty_r in *. applys P4. applys* hstar_intro.
+Qed.
+
+(* ----------------------------------------------------------------- *)
+(** *** Properties of qwand *)
+
+Lemma qwand_equiv : forall H A (Q1 Q2:A->hprop),
+  H ==> (Q1 \--* Q2) <-> (Q1 \*+ H) ===> Q2.
+Proof using.
+  unfold qwand. iff M.
+  { intros x. rewrite hstar_comm. applys himpl_hstar_trans_l (rm M).
+    applys himpl_trans. applys hstar_hforall. simpl.
+    applys himpl_hforall_l x. rewrite hstar_comm. applys hwand_cancel. }
+  { applys himpl_hforall_r. intros x. rewrite* hwand_equiv. }
+Qed.
+
+Lemma qwand_cancel : forall A (Q1 Q2:A->hprop),
+  Q1 \*+ (Q1 \--* Q2) ===> Q2.
+Proof using. intros. rewrite <- qwand_equiv. applys qimpl_refl. Qed.
+
+Lemma himpl_qwand_r : forall A (Q1 Q2:A->hprop) H,
+  Q1 \*+ H ===> Q2 ->
+  H ==> (Q1 \--* Q2).
+Proof using. introv M. rewrite~ qwand_equiv. Qed.
+
+Arguments himpl_qwand_r [A].
+
+Lemma qwand_specialize : forall A (x:A) (Q1 Q2:A->hprop),
+  (Q1 \--* Q2) ==> (Q1 x \-* Q2 x).
+Proof using. intros. applys* himpl_hforall_l x. Qed.
+
+Arguments qwand_specialize [ A ].
+
+(* ----------------------------------------------------------------- *)
+(** *** Properties of [htop] *)
+
+Lemma htop_intro : forall h,
+  \Top h.
+Proof using. intros. exists~ (=h). Qed.
+
+Lemma himpl_htop_r : forall H,
+  H ==> \Top.
+Proof using. intros. intros h Hh. applys* htop_intro. Qed.
+
+Lemma htop_eq :
+  \Top = (\exists H, H).
+Proof using. auto. Qed.
+
+Lemma hstar_htop_htop :
+  \Top \* \Top = \Top.
+Proof using.
+  applys himpl_antisym.
+  { applys himpl_htop_r. }
+  { rewrite <- hstar_hempty_r at 1. applys himpl_frame_r. applys himpl_htop_r. }
+Qed.
+
+(* ----------------------------------------------------------------- *)
+(** *** Properties of [hsingle] *)
+
+Lemma hsingle_intro : forall p v,
+  (p ~~> v) (Fmap.single p v).
+Proof using. intros. hnfs*. Qed.
+
+Lemma hsingle_inv: forall p v h,
+  (p ~~> v) h ->
+  h = Fmap.single p v.
+Proof using. auto. Qed.
+
+Lemma hstar_hsingle_same_loc : forall p w1 w2,
+  (p ~~> w1) \* (p ~~> w2) ==> \[False].
+Proof using.
+  intros. unfold hsingle. intros h (h1&h2&E1&E2&D&E). false.
+  subst. applys* Fmap.disjoint_single_single_same_inv.
+Qed.
+
+Arguments hstar_hsingle_same_loc : clear implicits.
+
+(* ----------------------------------------------------------------- *)
+(** *** Definition and Properties of [haffine] and [hgc] *)
+
+Definition haffine (H:hprop) :=
+  True.
+
+Lemma haffine_hany : forall (H:hprop),
+  haffine H.
+Proof using. unfold haffine. auto. Qed.
+
+Lemma haffine_hempty :
+  haffine \[].
+Proof using. applys haffine_hany. Qed.
+
+Definition hgc := (* equivalent to [\exists H, \[haffine H] \* H] *)
+  htop.
+
+Notation "\GC" := (hgc) : hprop_scope.
+
+Lemma haffine_hgc :
+  haffine \GC.
+Proof using. applys haffine_hany. Qed.
+
+Lemma himpl_hgc_r : forall H,
+  haffine H ->
+  H ==> \GC.
+Proof using. introv M. applys himpl_htop_r. Qed.
+
+Lemma hstar_hgc_hgc :
+  \GC \* \GC = \GC.
+Proof using. applys hstar_htop_htop. Qed.
+
+(* ----------------------------------------------------------------- *)
+(** *** Functor Instantiation to Obtain [xsimpl] *)
+
+End SepSimplArgs.
+
+(** We are now ready to instantiate the functor that defines [xsimpl].
+    Demos of [xsimpl] are presented in chapter [Himpl.v]. *)
+
+Module Export HS := LibSepSimpl.XsimplSetup(SepSimplArgs).
+
+Export SepSimplArgs.
+
+(** From now on, all operators have opaque definitions. *)
+
+Global Opaque hempty hpure hstar hsingle hexists hforall
+              hwand qwand htop hgc haffine.
+
+(** At this point, the tactic [xsimpl] is defined. There remains to customize
+    the tactic so that it recognizes the predicate [p ~~> v] in a special way
+    when performing simplifications. *)
+
+(** The tactic [xsimpl_hook_hsingle p v] operates as part of [xsimpl].
+    The specification that follows makes sense only in the context of the
+    presentation of the invariants of [xsimpl] described in [LibSepSimpl.v].
+    This tactic is invoked on goals of the form [Xsimpl (Hla, Hlw, Hlt) HR],
+    where [Hla] is of the form [H1 \* .. \* Hn \* \[]]. The tactic
+    [xsimpl_hook_hsingle p v] searches among the [Hi] for a heap predicate
+    of the form [p ~~> v']. If it finds one, it moves this [Hi] to the front,
+    just before [H1]. Then, it cancels it out with the [p ~~> v] that occurs
+    in [HR]. Otherwise, the tactic fails. *)
+
+Ltac xsimpl_hook_hsingle p :=
+  xsimpl_pick_st ltac:(fun H' =>
+    match H' with (hsingle p ?v') =>
+      constr:(true) end);
+  apply xsimpl_lr_cancel_eq;
+  [ xsimpl_lr_cancel_eq_repr_post tt | ].
+
+(** The tactic [xsimpl_hook] handles cancellation of heap predicates of the
+    form [p ~~> v]. It forces their cancellation against heap predicates of
+    the form [p ~~> w], by asserting the equality [v = w]. Note: this tactic
+    is later refined to also handle records. *)
+
+Ltac xsimpl_hook H ::=
+  match H with
+  | hsingle ?p ?v => xsimpl_hook_hsingle p
+  end.
+
+(** One last hack is to improve the [math] tactic so that it is able
+    to handle the [val_int] coercion in goals and hypotheses of the
+    form [val_int ?n = val_int ?m], and so that it is able to process
+    the well-founded relations [dowto] and [upto] for induction on
+    integers. *)
+
+(* Ltac math_0 ::=
+  unfolds downto, upto;
+  repeat match goal with
+  | |- val_int _ = val_int _ => fequal
+  | H: val_int _ = val_int _ |- _ => inverts H
+  end. *)
+
+(* ================================================================= *)
+(** ** Specification of Record Operations *)
+
+(** The chapter [Struct] shows how to these specifications may be
+    realized. *)
+
+Implicit Types k : nat.
+
+(* ----------------------------------------------------------------- *)
+(** *** Representation of Records *)
+
+(** A field name is implemented as a natural number *)
+
+Definition field : Type := nat.
+
+(** A record field is described as the pair of a field and a value stored
+    in that field. *)
+
+Definition hrecord_field : Type := (field * val).
+
+(** A record consists of a list of fields. *)
+
+Definition hrecord_fields : Type := list hrecord_field.
+
+Implicit Types kvs : hrecord_fields.
+
+(* end LibSepReference *)
+
+Lemma hstar_hpure_conj : forall H1 H2,
+  (\[H1] \* \[H2]) = \[H1 /\ H2].
+Proof.
+  intros.
+  apply fun_ext_dep. intros h.
+  rewrite hstar_hpure_l.
+  apply prop_ext.
+  split; intros.
+  { destruct H. apply hpure_inv in H0. destruct H0. subst. apply hpure_intro. intuition. }
+  { apply hpure_inv in H. destruct H as ((?&?)&?). subst. intuition. now apply hpure_intro. }
+Qed.
+
+Ltac hinv H :=
+  match type of H with
+  | \[] _ => apply hempty_inv in H
+  | \[_] _ => apply hpure_inv in H as (?&?)
+  | (_~~>_) _ => apply hsingle_inv in H
+  | (_ \* _) _ => apply hstar_inv in H as (?&?&?&?&?&?)
+  | (\[_] \* _) _ => rewrite hstar_hpure_l
+  | (_ \* \[_]) _ => rewrite hstar_hpure_r
+  end.
+
+Ltac hintro :=
+  match goal with
+  | |- \[] _ => apply hempty_intro
+  | |- \[_] _ => apply hpure_intro
+  | |- (_ \* _) (_ \u _) => apply hstar_intro
+  | |- (\[_] \* _) _ => rewrite hstar_hpure_l
+  | |- (_ \* \[_]) _ => rewrite hstar_hpure_r
+  end.
+
+End HeapSetup.
